full-simpl/test.v
@@ -1,0 +1,848 @@
+Require Coq.extraction.Extraction.
+Require Import Ascii String Coq.Strings.Byte.
+Require Export ExtrOcamlChar.
+Extract Inductive bool => "bool" ["true" "false"].
+Extract Inductive string => "char list" [ "[]" "(::)" ].
+From Coq Require Import Lists.List.
+Extract Inductive list => "list" [ "[]" "(::)" ].
+Extraction Language OCaml.
+Import ListNotations.
+Load "../std".
+
+Module deBruijin.
+
+Module E11_1.
+
+Inductive ty : Type :=
+| Bool
+| Arrow (T1 T2: ty)
+| Unit.
+Notation "t1 '|-->' t2" := (Arrow t1 t2) (at level 40).
+
+Inductive term : Type :=
+(*純粋λ計算*)
+| var (n: nat)
+| abs (name: string) (typ: ty) (t: term)
+| app (t1 t2: term)
+
+(*ぶーる*)
+| tru
+| fls
+| If (t1 t2 t3: term)
+(*拡張*)
+| unit
+| seq (t1 t2: term).
+
+Inductive value : term -> Prop :=
+  | v_abs : forall x T t, value (abs x T t)
+  | v_tru : value tru
+  | v_fls : value fls
+  | v_unit: value unit.
+
+Definition isval t :=
+  match t with
+  | tru => true
+  | fls => true
+  | abs _ _ _ => true
+  | unit => true
+  | _ => false
+  end.
+
+Fixpoint eqb_ty (T1 T2: ty) : bool :=
+  match (T1, T2) with
+  | (Bool, Bool) => true
+  | (Unit, Unit) => true
+  | (T11 |--> T12, T21 |--> T22) =>
+    andb (eqb_ty T11 T21) (eqb_ty T12 T22)
+  | _ => false
+  end.
+
+Lemma eq_type_refl : forall T,
+    eqb_ty T T = true.
+Proof.
+  induction T; simpl; auto. rewrite IHT1, IHT2; auto.
+Qed.
+
+Definition context := list (string * ty).
+Definition eqb_string s1 s2:= String.eqb s1 s2.
+
+Fixpoint getbinding (n : nat) (ctx: context) :=
+  match n with
+  | 0 =>
+    match ctx with
+    | [] => None
+    | (x, t) :: ctx' => Some t
+    end
+  | S n' =>
+    match ctx with
+    | [] => None
+    | x :: ctx' => getbinding n' ctx'
+    end
+  end.
+
+Fixpoint shift (c : nat) (t : term) : term :=
+match t with
+| var x => var (if leb c x then (S x) else x)
+| abs x T t' => abs x T (shift (S c) t')
+| app t1 t2 => app (shift c t1) (shift c t2)
+| tru => tru
+| fls => fls
+| If t1 t2 t3 => If (shift c t1) (shift c t2) (shift c t3)
+| unit => unit
+| seq t1 t2 => seq (shift c t1) (shift c t2)
+end.
+
+Fixpoint unshift (c : nat) (t : term) : term :=
+match t with
+| var x => var (if leb c x then (pred x) else x)
+| abs x T t' => abs x T (unshift (S c) t')
+| app t1 t2 => app (unshift c t1) (unshift c t2)
+| tru => tru
+| fls => fls
+| If t1 t2 t3 => If (unshift c t1) (unshift c t2) (unshift c t3)
+| unit => unit
+| seq t1 t2 => seq (unshift c t1) (unshift c t2)
+end.
+
+Fixpoint subst (d : nat) (s t: term) : term :=
+match t with
+| var x =>
+  if eqb_nat d x then s
+  else t
+| abs x T t' => abs x T (subst (S d) s t')
+| app t1 t2 => app (subst d s t1) (subst d s t2)
+| If t1 t2 t3 =>
+  If (subst d s t1) (subst d s t2) (subst d s t3)
+| seq t1 t2 =>
+  seq (subst d s t1) (subst d s t2)
+| _ => t
+end.
+
+Fixpoint shift_S (d k : nat) (t : term) : term :=
+match t with
+| var x => var (if leb d x then x + k else x)
+| abs x T t' => abs x T (shift_S (S d) k t')
+| app t1 t2 => app (shift_S d k t1) (shift_S d k t2)
+| tru => tru
+| fls => fls
+| If t1 t2 t3 =>
+  If (shift_S d k t1) (shift_S d k t2) (shift_S d k t3)
+| unit => unit
+| seq t1 t2 =>
+  seq (shift_S d k t1) (shift_S d k t2)
+end.
+
+Lemma PM_shift : forall t n,
+    unshift n (shift n t) = t.
+Proof.
+  induction t; simpl; intros; auto.
+  -
+    destruct (leb n0 n) eqn:IH1.
+    apply le_leb in IH1. apply le_S in IH1. apply leb_le in IH1. rewrite IH1. simpl. reflexivity.
+    rewrite IH1. reflexivity.
+  -
+    rewrite IHt. reflexivity.
+  -
+    rewrite IHt1, IHt2; reflexivity.
+  -
+    rewrite IHt1, IHt2, IHt3; reflexivity.
+  -
+    rewrite IHt1, IHt2; reflexivity.
+Qed.
+
+Fixpoint subst_s (d : nat) (s t: term) : term :=
+match t with
+| var x =>
+  if eqb_nat d x then
+    s
+  else
+    if ltb d x then
+      var (pred x) else var x
+| abs x T t' => abs x T (subst_s (S d) s t')
+| app t1 t2 => app (subst_s d s t1) (subst_s d s t2)
+| tru => tru
+| fls => fls
+| unit => unit
+| If t1 t2 t3 =>
+  If (subst_s d s t1) (subst_s d s t2) (subst_s d s t3)
+| seq t1 t2 =>
+  seq (subst_s d s t1) (subst_s d s t2)
+end.
+
+Lemma sub_S : forall t1 t2 n,
+unshift n (subst n (shift n t2) t1) = subst_s n t2 t1.
+Proof.
+  induction t1; simpl; intros; auto.
+  destruct eqb_nat eqn:H. rewrite PM_shift. reflexivity.
+  simpl. destruct ltb eqn:IH1. apply ltb_to_leb in IH1. rewrite IH1. reflexivity.
+  destruct leb eqn:IH2. apply leb_neq_lt in IH2; auto. rewrite IH1 in IH2. inversion IH2.
+  reflexivity.
+
+  rewrite <- IHt1. admit.
+  rewrite IHt1_1, IHt1_2; reflexivity.
+  rewrite IHt1_1, IHt1_2, IHt1_3; reflexivity.
+  rewrite IHt1_1, IHt1_2; reflexivity.
+Abort.
+
+
+Reserved Notation " t '-->i' t' " (at level 40).
+Inductive internal_step :term -> term -> Prop :=
+| Ei_IfTrue : forall t2 t3,
+    If tru t2 t3 -->i t2
+| Ei_IfFalse : forall t2 t3,
+    If fls t2 t3 -->i t3
+| Ei_If : forall t1 t1' t2 t3,
+    t1 -->i t1' ->
+    If t1 t2 t3 -->i If t1' t2 t3
+| Ei_App1 : forall t1 t2 t1',
+    t1 -->i t1' ->
+    app t1 t2 -->i app t1' t2
+| Ei_App2 : forall v1 t2 t2',
+    value v1 ->
+    t2 -->i t2' ->
+    app v1 t2 -->i app v1 t2'
+| Ei_AppAbs : forall typ str t12 t2,
+    value t2 ->
+    app (abs str typ t12) t2 -->i unshift 0 (subst 0 (shift 0 t2) t12)
+
+where " t '-->i' t' " := (internal_step t t').
+
+Reserved Notation " t '-->e' t' " (at level 40).
+Inductive external_step : term -> term -> Prop :=
+| E_IfTrue : forall t2 t3,
+    If tru t2 t3 -->e t2
+| E_IfFalse : forall t2 t3,
+    If fls t2 t3 -->e t3
+| E_If : forall t1 t1' t2 t3,
+    t1 -->e t1' ->
+    If t1 t2 t3 -->e If t1' t2 t3
+| E_App1 : forall t1 t2 t1',
+    t1 -->e t1' ->
+    app t1 t2 -->e app t1' t2
+| E_App2 : forall v1 t2 t2',
+    value v1 ->
+    t2 -->e t2' ->
+    app v1 t2 -->e app v1 t2'
+| E_AppAbs : forall typ str t12 t2,
+    value t2 ->
+    app (abs str typ t12) t2 -->e unshift 0 (subst 0 (shift 0 t2) t12)
+| E_seq : forall t1 t1' t2,
+    t1 -->e t1' ->
+    seq t1 t2 -->e seq t1' t2
+| E_SeqNext : forall v1 t2,
+    value v1 ->
+    seq v1 t2 -->e t2
+where " t '-->e' t' " := (external_step t t').
+
+
+Lemma shift_sub : forall t1 t2 n,
+unshift n (subst n (shift n t2) (shift n t1)) = t1.
+Proof.
+  induction t1; intros; simpl; auto.
+  destruct leb eqn:IH1. destruct eqb_nat eqn:IH2. apply eqb_eq in IH2. subst.
+  generalize Nat.nle_succ_diag_l. intros. apply le_leb in IH1. specialize (H n). induction H. apply IH1.
+  simpl. rewrite IH2. rewrite IH1. reflexivity.
+  destruct eqb_nat eqn:IH2. apply eqb_eq in IH2. subst. rewrite leb_refl in IH1. inversion IH1.
+  simpl. rewrite IH1. reflexivity.
+  (* rewrite IHt1. reflexivity. *)
+  admit.
+  rewrite IHt1_1; rewrite IHt1_2; reflexivity.
+  rewrite IHt1_1, IHt1_2, IHt1_3; reflexivity.
+  rewrite IHt1_1, IHt1_2. reflexivity.
+Abort.
+
+Fixpoint e2t t :=
+  match t with
+  | var x => var x
+  | abs x T t' => abs x T (e2t t')
+  | app t1 t2 => app (e2t t1) (e2t t2)
+  | If t1 t2 t3 => If (e2t t1) (e2t t2) (e2t t3)
+  | seq t1 t2 => app (abs "x" Unit (shift 0 (e2t t2))) (e2t t1)
+  | _ => t
+  end.
+
+Lemma shift_sub_1 : forall t1 t2 n,
+    unshift n (subst n (shift 0 t2) (shift n t1)) = t1.
+Proof.
+  induction t1; simpl; intros; auto.
+  destruct (leb n0 n) eqn:IH1.
+  destruct eqb_nat eqn:IH2. apply eqb_eq in IH2. subst.
+  generalize Nat.nle_succ_diag_l; intros. specialize (H n). apply leb_F in H.
+  rewrite H in IH1; inversion IH1.
+  simpl. rewrite IH2. rewrite IH1. reflexivity.
+  destruct eqb_nat eqn:IH2. apply eqb_eq in IH2; subst.
+  rewrite leb_refl in IH1; inversion IH1.
+  simpl. rewrite IH1. reflexivity.
+
+  rewrite IHt1. reflexivity.
+  rewrite IHt1_1, IHt1_2; reflexivity.
+  rewrite IHt1_1, IHt1_2, IHt1_3; reflexivity.
+  rewrite IHt1_1, IHt1_2; reflexivity.
+Qed.
+
+Lemma subsub : forall t1 t2 n,
+    e2t (subst n t2 t1) = subst n (e2t t2) (e2t t1).
+Proof.
+  induction t1; simpl; intros; auto.
+
+  destruct eqb_nat; auto.
+  rewrite IHt1; reflexivity.
+  rewrite IHt1_1, IHt1_2; reflexivity.
+  rewrite IHt1_1, IHt1_2, IHt1_3; reflexivity.
+  rewrite IHt1_1, IHt1_2.
+
+
+
+Lemma dekinai : forall t n,
+    shift 0 (shift n t) = shift (S n) (shift 0 t).
+Proof.
+  induction t; simpl; intros; auto.
+  repeat rewrite leb0.
+  admit.
+Abort.
+
+Lemma shift_e2t : forall t n,
+    e2t (shift n t) = shift n (e2t t).
+Proof.
+  induction t; simpl; intros; auto.
+  rewrite IHt. reflexivity.
+  rewrite IHt1, IHt2; reflexivity.
+  rewrite IHt1, IHt2, IHt3; reflexivity.
+  rewrite IHt1. rewrite IHt2.
+Abort.
+
+Theorem T11_3_1_1_1 : forall t t',
+  t -->e t' ->
+  (e2t t) -->i (e2t t').
+Proof.
+  induction t; intros; simpl; try solve_by_inverts 2.
+  -
+    inversion H; subst; simpl; try constructor; auto.
+    +
+      destruct t1; try solve_by_invert; constructor.
+    +
+      admit.
+  -
+    inversion H; subst; simpl; try constructor; auto.
+  -
+    inversion H; subst; simpl; try constructor; auto; try solve_by_invert.
+    +
+      constructor.
+    +
+      remember (shift 0 (e2t t')) as s.
+      rewrite <- (shift_sub_1 (e2t t') (e2t t1) 0).
+      subst.
+      constructor. destruct t1; try solve_by_invert; constructor.
+Qed.
+
+Theorem T11_3_1_1_2 : forall t u,
+  (e2t t) -->i u ->
+  exists t', u = e2t t' /\ t -->e t'.
+Proof.
+  induction t; simpl; intros; try solve_by_invert.
+  -
+    inversion H; subst; simpl; try constructor.
+    +
+      apply IHt1 in H3; destruct H3; destruct H0; subst. exists (app x t2); split; try constructor; auto.
+    +
+      apply IHt2 in H4; destruct H4; destruct H0; subst. exists (app t1 x); split; try constructor; auto.
+      destruct t1; try solve_by_invert; constructor.
+    +
+      destruct t1; try solve_by_invert. simpl in H0. inversion H0; subst.
+      exists (subst 0 t2 t1). split. symmetry. rewrite sub_e2t.
+      constructor. destruct t2; try solve_by_invert; constructor.
+  -
+    inversion H; subst.
+    +
+      destruct t1; try solve_by_invert. simpl in H1. exists t2. split; auto; constructor.
+    +
+      destruct t1; try solve_by_invert. simpl in H1. exists t3; split; auto; constructor.
+    +
+      apply IHt1 in H4. destruct H4; destruct H0; subst.
+      exists (If x t2 t3); split; try constructor; auto.
+  -
+    inversion H; subst.
+    +
+      subst. inversion H3.
+    +
+      apply IHt1 in H4. destruct H4; destruct H0; subst. exists (seq x t2); split; try constructor; auto.
+    +
+      exists t2. split; try constructor; auto. apply shift_sub. destruct t1; try solve_by_invert; constructor.
+Qed.
+
+
+Reserved Notation "ctx '|-' t '\in' T" (at level 40).
+Inductive has_type : context -> term -> ty -> Prop :=
+| T_True: forall ctx,
+      ctx |- tru \in Bool
+| T_False: forall ctx,
+      ctx |- fls \in Bool
+| T_If: forall ctx t1 t2 t3 T',
+      ctx |- t1 \in Bool ->
+      ctx |- t2 \in T' ->
+      ctx |- t3 \in T' ->
+      ctx |- (If t1 t2 t3) \in T'
+| T_Var: forall ctx n1 t,
+      getbinding n1 ctx = Some t ->
+      ctx |- (var n1) \in t
+| T_Abs: forall ctx x T1 t2 T2,
+      ((x, T1) :: ctx) |- t2 \in T2 ->
+      ctx |- (abs x T1 t2) \in (T1 |--> T2)
+| T_App: forall ctx t1 T11 T12 t2,
+      ctx |- t1 \in (T11 |--> T12) ->
+      ctx |- t2 \in T11 ->
+      ctx |- app t1 t2 \in T12
+| T_Unit: forall ctx,
+    ctx |- unit \in Unit
+| T_Seq : forall ctx t1 t2 T2,
+    ctx |- t1 \in Unit ->
+    ctx |- t2 \in T2 ->
+    ctx |- (seq t1 t2) \in T2
+
+where " ctx '|-' x '\in' t " := (has_type ctx x t).
+
+Lemma appGetbind : forall ctx ctx' n,
+    getbinding (n + (length ctx)) (ctx ++ ctx') = getbinding n ctx'.
+Proof.
+  induction ctx; simpl; intros; auto.
+  rewrite <- plus_n_O; reflexivity.
+  rewrite <- plus_Snm_nSm. simpl. apply IHctx.
+Qed.
+
+Lemma length1_Some : forall n ctx ctx1 ctx2 T,
+    n < length ctx ->
+    getbinding n (ctx ++ ctx1) = Some T ->
+    getbinding n (ctx ++ ctx2) = Some T.
+Proof.
+  induction n; simpl; intros. destruct ctx. inversion H. simpl. simpl in H0. apply H0.
+  destruct ctx. inversion H. simpl. destruct ( (p :: ctx) ++ ctx1) eqn:IHH. inversion H0. inversion IHH; subst.
+  eapply IHn in H0. apply H0. simpl in H. apply lt_S_n in H. apply H.
+Qed.
+
+Lemma shifting : forall t g g1 g2 T,
+  (g1 ++ g) |- t \in T ->
+  (g1 ++ g2 ++ g) |- (shift (length g1) (length g2) t) \in T.
+Proof.
+  induction t; intros; inversion H; subst; clear H; try solve [econstructor; eauto]; simpl.
+
+  apply T_Var. destruct (leb) eqn:IH. apply le_leb in IH.
+  generalize dependent g. generalize dependent T. generalize dependent n.
+  induction g1; simpl; intros; eauto. unfold getbinding. rewrite appGetbind. apply H2.
+  destruct n. inversion IH. simpl.
+  apply le_S_n in IH. simpl in H2. eapply IHg1 in IH; eauto.
+
+  apply leb_neq in IH. eapply length1_Some in IH. apply IH. apply H2.
+
+  apply T_Abs.
+  assert (S (length g1) = length ((name, typ) :: g1)). reflexivity.
+  rewrite H. apply IHt with (g1:= ((name, typ) :: g1)). apply H5.
+Qed.
+
+Lemma shifting_l : forall t g g1 g2 T,
+  (g1 ++ g2 ++ g) |- (shift (length g1) (length g2) t) \in T ->
+  (g1 ++ g) |- t \in T.
+Proof.
+  induction t; intros; inversion H; subst; clear H; try solve [econstructor; eauto]; simpl.
+  -
+    apply T_Var. destruct (leb) eqn:IH. apply le_leb in IH.
+    generalize dependent g. generalize dependent T. generalize dependent n.
+    induction g1; simpl; intros; eauto. unfold getbinding in H2. rewrite appGetbind in H2. apply H2.
+    destruct n. inversion IH. simpl.
+    apply le_S_n in IH. simpl in H2. eapply IHg1 in IH; eauto.
+    apply leb_neq in IH. eapply length1_Some in IH. apply IH. apply H2.
+  -
+    apply T_Abs.
+    assert (S (length g1) = length ((name, typ) :: g1)). reflexivity. rewrite H in H5.
+    eapply IHt with (g1:= ((name, typ) :: g1)). apply H5.
+Qed.
+
+Theorem T11_3_1_2 : forall t T ctx,
+    ctx |- t \in T <->
+    ctx |- (e2t t) \in T.
+Proof.
+  split; generalize dependent T; generalize dependent ctx.
+  -
+    induction t; simpl; intros; auto; inversion H; subst; try solve [econstructor; eauto].
+    +
+      econstructor. constructor; auto.
+      assert (("x"%string, Unit) :: ctx = [] ++ [("x"%string, Unit)] ++ ctx). reflexivity. rewrite H0.
+      apply shifting. simpl. apply IHt2. apply H5.
+      apply IHt1. apply H3.
+  -
+    induction t; simpl; intros; inversion H; subst; try solve [econstructor; eauto].
+    inversion H3; subst. apply T_Seq. apply IHt1. apply H5. apply IHt2.
+    assert (ctx = [] ++ ctx). reflexivity. rewrite H0.
+    eapply shifting_l with (g2:= [("x"%string, Unit)]).
+    assert ([] ++ [("x"%string, Unit)] ++ ctx = [("x"%string, Unit)] ++ ctx). reflexivity.
+    apply H2.
+Qed.
+
+End E11_1.
+
+End deBruijin.
+
+Module string.
+
+Module Seq.
+Inductive ty : Type :=
+| Bool
+| Unit
+|Arrow (ty1 ty2: ty) .
+Notation "t1 '|-->' t2" := (Arrow t1 t2) (at level 40).
+
+Inductive term : Type :=
+(*純粋λ計算*)
+| var (name: string)
+| abs (name: string) (typ: ty) (t: term)
+| app (t1 t2: term)
+(*ぶーる*)
+| tru
+| fls
+| unit
+| If (t1 t2 t3: term)
+| seq (t1 t2: term).
+
+Inductive value : term -> Prop :=
+  | v_abs : forall x T t, value (abs x T t)
+  | v_tru : value tru
+  | v_fls : value fls
+  | v_uni : value unit.
+
+Reserved Notation "'[' x ':=' s ']' t" (at level 20).
+
+Fixpoint subst (x : string) (s : term) (t : term) : term :=
+  match t with
+  | var x' => if String.eqb x x' then s else t
+  | abs x' T t1 => abs x' T (if String.eqb x x' then t1 else ([x:=s] t1))
+  | app t1 t2 => app ([x:=s] t1) ([x:=s] t2)
+  | tru => tru
+  | fls => fls
+  | unit => unit
+  | If t1 t2 t3 => If ([x:=s] t1) ([x:=s] t2) ([x:=s] t3)
+  | seq t1 t2 => seq ([x:=s]t1) ([x:=s]t2)
+  end
+
+where "'[' x ':=' s ']' t" := (subst x s t).
+
+Reserved Notation "t1 '-->' t2" (at level 40).
+
+Inductive step : term -> term -> Prop :=
+  | E_AppAbs : forall x T t12 v2,
+         value v2 ->
+         (app (abs x T t12) v2) --> [x:=v2]t12
+  | E_App1 : forall t1 t1' t2,
+         t1 --> t1' ->
+         app t1 t2 --> app t1' t2
+  | E_App2 : forall v1 t2 t2',
+         value v1 ->
+         t2 --> t2' ->
+         app v1 t2 --> app v1 t2'
+  | E_IfTru : forall t1 t2,
+      (If tru t1 t2) --> t1
+  | E_IfFls : forall t1 t2,
+      (If fls t1 t2) --> t2
+  | E_If : forall t1 t1' t2 t3,
+      t1 --> t1' ->
+      (If t1 t2 t3) --> (If t1' t2 t3)
+  | E_seq : forall t1 t1' t2,
+      t1 --> t1' ->
+      seq t1 t2 --> seq t1' t2
+  | E_SeqNext : forall v1 t2,
+      value v1 ->
+      seq v1 t2 --> t2
+
+where "t1 '-->' t2" := (step t1 t2).
+
+
+Definition context := partial_map ty.
+
+Inductive ctx_no : context -> string -> string -> Prop :=
+  | ctx_some : forall ctx x T,
+      ctx x = Some T ->
+      ctx_no ctx x (append x "'")
+  | ctx_none : forall ctx x,
+      ctx x = None ->
+      ctx_no ctx x x.
+
+
+Lemma ctx_no_det : forall x ctx x' x'',
+    ctx_no ctx x x' ->
+    ctx_no ctx x x'' ->
+    ctx x' = None -> ctx x'' = None ->
+    x' = x''.
+Proof.
+  intros. generalize dependent x''.
+  induction H; intros; auto.
+  inversion H0; subst. reflexivity.
+  rewrite H in H2. inversion H2.
+  induction H0; auto.
+  rewrite H in H0. inversion H0.
+Qed.
+
+Inductive appears_free_in : string -> term -> Prop :=
+  | afi_var : forall x,
+      appears_free_in x (var x)
+  | afi_app1 : forall x t1 t2,
+      appears_free_in x t1 ->
+      appears_free_in x (app t1 t2)
+  | afi_app2 : forall x t1 t2,
+      appears_free_in x t2 ->
+      appears_free_in x (app t1 t2)
+  | afi_abs : forall x y T11 t12,
+      y <> x ->
+      appears_free_in x t12 ->
+      appears_free_in x (abs y T11 t12)
+  | afi_test1 : forall x t1 t2 t3,
+      appears_free_in x t1 ->
+      appears_free_in x (If t1 t2 t3)
+  | afi_test2 : forall x t1 t2 t3,
+      appears_free_in x t2 ->
+      appears_free_in x (If t1 t2 t3)
+  | afi_test3 : forall x t1 t2 t3,
+      appears_free_in x t3 ->
+      appears_free_in x (If t1 t2 t3)
+  | afi_seq1 : forall x t1 t2,
+      appears_free_in x t1 ->
+      appears_free_in x (seq t1 t2)
+  | afi_seq2 : forall x t1 t2,
+      appears_free_in x t2 ->
+      appears_free_in x (seq t1 t2).
+
+Fixpoint free x t :=
+  match t with
+  | var x' => eqb x x'
+  | app t1 t2 =>
+    orb (free x t1) (free x t2)
+  | abs y T t1 =>
+    if eqb x y then false
+    else free x t1
+  | If t1 t2 t3 =>
+    (free x t1) || (free x t2) || (free x t3)
+  | tru => false
+  | fls => false
+  | unit => false
+  | seq t1 t2 =>
+    (free x t1) || (free x t2)
+  end.
+
+
+Inductive free_name : term -> string -> string -> Prop :=
+  | free_x : forall x t,
+      free x t = true ->
+      free_name t x (append x "'")
+  | not_free : forall x t,
+      free x t = false ->
+      free_name t x x.
+
+Lemma name_det : forall x x1 x2 t,
+    free_name t x x1 ->
+    free_name t x x2 ->
+    x1 = x2.
+Proof.
+  intros. generalize dependent x2; induction H; intros;
+  induction H0; auto; rewrite H in H0; inversion H0.
+Qed.
+
+Inductive multi_name : term -> string -> string -> Prop :=
+| name_refl : forall x t,
+    multi_name t x x
+| name_malti : forall t x1 x2 x3,
+    free_name t x1 x2 ->
+    free_name t x2 x3 ->
+    multi_name t x1 x3.
+
+Lemma multi_det : forall t x x1 x2,
+    multi_name t x x1 -> multi_name t x x2 ->
+    free x1 t = false -> free x2 t = false ->
+    x1 = x2.
+Proof.
+  intros. generalize dependent x2. induction H; intros.
+  inversion H0; subst; auto.
+  admit.
+  admit.
+Admitted.
+
+
+Inductive e2t : term -> context -> term -> Prop :=
+| evar : forall x ctx, e2t (var x) ctx (var x)
+| eabs : forall x T t t' ctx,
+    e2t t ctx t' ->
+    e2t (abs x T t) ctx (abs x T t')
+| eapp : forall t1 t2 t1' t2' ctx,
+    e2t t1 ctx t1' -> e2t t2 ctx t2' ->
+    e2t (app t1 t2) ctx (app t1' t2')
+| etru : forall ctx,
+    e2t tru ctx tru
+| efls : forall ctx,
+    e2t fls ctx fls
+| eunit : forall ctx,
+    e2t unit ctx unit
+| eif : forall ctx t1 t2 t3 t1' t2' t3',
+    e2t t1 ctx t1' -> e2t t2 ctx t2' -> e2t t3 ctx t3' ->
+    e2t (If t1 t2 t3) ctx (If t1' t2' t3')
+| eseq : forall x ctx t1 t2 t1' t2',
+    free_name (seq t1 t2) "x" x ->
+    e2t t1 ctx t1' -> e2t t2 ctx t2' ->
+    e2t (seq t1 t2) ctx (app (abs x Unit t2') t1').
+
+Lemma e2t_det : forall t t1 t2 ctx1 ctx2,
+    e2t t ctx1 t1 ->
+    e2t t ctx2 t2 ->
+    t1 = t2.
+Proof.
+  induction t; simpl; intros; inversion H; inversion H0; subst; auto .
+  erewrite IHt with (t1:= t'); eauto.
+  erewrite IHt1 with (t2:= t1'); eauto. erewrite IHt2 with (t1:= t2'); eauto.
+  erewrite IHt1 with (t2:= t1'); eauto. erewrite IHt2 with (t1:= t2'); eauto. erewrite IHt3 with (t1:= t3'); eauto.
+  erewrite IHt2 with (t1:= t2'); eauto. erewrite IHt1 with (t2:= t1'); eauto.
+  erewrite name_det with (x1:= x); eauto.
+Qed.
+
+Lemma sub_E : forall t12 t2 n ctx t2' t12',
+    e2t t2 ctx t2' -> e2t t12 ctx t12' ->
+    e2t (subst n t2 t12) ctx (subst n t2' t12').
+Proof.
+  induction t12; simpl; intros; inversion H0; subst; simpl; eauto; try solve [inversion H1; subst; auto].
+  destruct eqb; auto.
+  destruct eqb; eauto. apply eabs; auto.
+  apply eapp; auto.
+  apply eif; auto.
+  destruct eqb; auto.
+  admit.
+
+  inversion H0; subst.
+  apply eseq; auto.
+  destruct (free "x" (seq ([n := t2] t12_1) ([n:= t2] t12_2) )) eqn:IH.
+
+Admitted.
+
+Theorem T11_3_1_1 : forall t t' ctx t1 t1',
+  t --> t' ->
+  e2t t ctx t1 -> e2t t' ctx t1' ->
+  t1 --> t1'.
+Proof.
+  intros. generalize dependent t1; generalize dependent t1'.
+  induction H; intros.
+
+  -
+    inversion H0; subst. inversion H4; subst.
+    eapply sub_E with (n:= x) in H7; eauto. eapply e2t_det with (t2:= t1') in H7; eauto. subst. apply E_AppAbs.
+
+
+
+  induction t; intros; try solve_by_invert.
+  -
+    inversion H0; subst. inversion H; subst.
+    inversion H4; subst. eapply sub_E with (n:= x) in H1; eauto. erewrite e2t_det with (t:= ()). apply E_AppAbs; auto.
+    inversion H6; subst; destruct t2'; try solve_by_invert; constructor.
+
+    inversion H1; subst. eapply e2t_det in H7; eauto; subst. apply E_App1; auto.
+    eapply IHt1; eauto.
+
+    inversion H1; subst.
+    eapply e2t_det in H4; eauto; subst. apply E_App2; auto.
+    inversion H5; subst; inversion H6; subst; constructor.
+    eapply IHt2; eauto.
+  -
+    inversion H0; subst. inversion H; subst.
+    inversion H5; subst. eapply e2t_det in H1; eauto; subst; constructor.
+    inversion H5; subst. eapply e2t_det in H1; eauto; subst; constructor.
+
+    inversion H1; subst. eapply e2t_det in H8; eauto; subst. eapply e2t_det in H9; eauto; subst.
+    apply E_If. eapply IHt1; eauto.
+  -
+    inversion H0; subst.
+    eapply e2t_det in H5; eauto; subst.
+    eapply name_det in H4; eauto; subst. eapply e2t_det in H8; eauto; subst. apply E_App2.
+    constructor. eapply IHt1; eauto.
+
+    eapply e2t_det in H1; eauto; subst.
+    rewrite <- (value_subst t1' t1'0 x).
+    assert (abs x Unit ([x := t1'0]t1') = abs x Unit t1').
+    rewrite (value_subst t1' t1'0 x). reflexivity.
+    admit.
+    rewrite H1.
+    apply E_AppAbs. inversion H8; subst; inversion H6; subst; constructor.
+    admit.
+Admitted.
+
+Open Scope string.
+
+Reserved Notation "ctx '|-' t '\in' T" (at level 40).
+Inductive has_type : context -> term -> ty -> Prop :=
+  | T_Var : forall ctx x T,
+      ctx x = Some T ->
+      ctx |- var x \in T
+  | T_Abs : forall ctx x T11 T12 t12,
+      (x |-> T11 ; ctx) |- t12 \in T12 ->
+      ctx |- abs x T11 t12 \in Arrow T11 T12
+  | T_App : forall T11 T12 ctx t1 t2,
+      ctx |- t1 \in Arrow T11 T12 ->
+      ctx |- t2 \in T11 ->
+      ctx |- app t1 t2 \in T12
+  | T_Tru : forall ctx,
+       ctx |- tru \in Bool
+  | T_Fls : forall ctx,
+       ctx |- fls \in Bool
+  | T_If : forall t1 t2 t3 T ctx,
+       ctx |- t1 \in Bool ->
+       ctx |- t2 \in T ->
+       ctx |- t3 \in T ->
+       ctx |- If t1 t2 t3 \in T
+
+where "ctx '|-' t '\in' T" := (has_type ctx t T).
+
+
+Reserved Notation "ctx '|-e' t '\in' T" (at level 40).
+Inductive ehas_type : context -> Eterm -> ty -> Prop :=
+  | eT_Var : forall ctx x T,
+      ctx x = Some T ->
+      ctx |-e Var x \in T
+  | eT_Abs : forall ctx x T11 T12 t12,
+      (x |-> T11 ; ctx) |-e t12 \in T12 ->
+      ctx |-e Abs x T11 t12 \in Arrow T11 T12
+  | eT_App : forall T11 T12 ctx t1 t2,
+      ctx |-e t1 \in Arrow T11 T12 ->
+      ctx |-e t2 \in T11 ->
+      ctx |-e App t1 t2 \in T12
+  | eT_Tru : forall ctx,
+       ctx |-e Tru \in Bool
+  | eT_Fls : forall ctx,
+       ctx |-e Fls \in Bool
+  | eT_If : forall t1 t2 t3 T ctx,
+       ctx |-e t1 \in Bool ->
+       ctx |-e t2 \in T ->
+       ctx |-e t3 \in T ->
+       ctx |-e EIf t1 t2 t3 \in T
+  | eT_Seq : forall ctx t1 t2 T2,
+      ctx |-e t1 \in Unit ->
+      ctx |-e t2 \in T2 ->
+      ctx |-e seq t1 t2 \in T2
+
+where "ctx '|-e' t '\in' T" := (ehas_type ctx t T).
+
+
+Theorem T11_3_1_2 : forall t ctx t' T,
+    e2t t ctx t' ->
+    ctx |-e t \in T <-> ctx |- t' \in T.
+Proof.
+  split;
+  generalize dependent t'; generalize dependent T; generalize dependent ctx;
+  induction t; intros; inversion H; subst; inversion H0; subst; auto; try solve [constructor; auto].
+
+  eapply T_App; eauto.
+
+  eapply T_App; eauto. apply T_Abs; auto.
+
+
+  generalize dependent t'. generalize dependent T. generalize dependent ctx.
+  induction t; intros; inversion H; subst; inversion H0; subst; auto; try solve [constructor; auto].
+
+  apply eT_Abs; auto. eapply IHt in H7; eauto. admit.
+
+
+
+
+End Seq.
+
+End string.
